fixed bugs in FindPrefixST and RangeST

examples/QueryStructure/Photoalbum.v
@@ -3,39 +3,28 @@ Require Import ADTSynthesis.QueryStructure.Automation.AutoDB
         ADTSynthesis.QueryStructure.Specification.SearchTerms.ListInclusion
         ADTSynthesis.QueryStructure.Specification.SearchTerms.InRange.
 
-(* Collection of Photos. Each photo contains the owner, the list of tags, and
-   the geolocation (latitude and longitude) *)
+Definition PHOTOS := "Photos".
+Definition PEOPLE := "Places".
 
-Definition PHOTOS := "Album".
-Definition USERS := "Users".
-
-Definition USER_ID := "UserId".
 Definition IMAGE_DATA := "ImageData".
 Definition TAGS := "Tags".
-Definition LATITUDE := "Latitude".
-Definition LONGITUDE := "Longitude".
 Definition NAME := "Name".
+Definition AGE := "Age".
 
 (* Represents image data by a list of byte characters *)
 Definition DataT := list ascii.
 
-(* Represents a natural number range by a pair of natural numbers *)
-Definition NatRange := prod nat nat.
-
 Definition AlbumSchema :=
   Query Structure Schema
     [ relation PHOTOS has
-               schema <USER_ID :: nat,
-                       IMAGE_DATA :: DataT,
+               schema <IMAGE_DATA :: DataT,
                        TAGS :: list string,
-                       LATITUDE :: nat,
-                       LONGITUDE :: nat>;
-      relation USERS has
-               schema <USER_ID :: nat,
-                       NAME :: string>
-                       where attributes [NAME] depend on [USER_ID]
+                       NAME :: string>;
+      relation PEOPLE has
+               schema <NAME :: string,
+                       AGE :: nat>
     ]
-    enforcing [attribute USER_ID  for PHOTOS references USERS].
+    enforcing [attribute NAME for PHOTOS references PEOPLE].
 
 Definition AlbumSig : ADTSig :=
   ADTsignature {
@@ -43,14 +32,12 @@ Definition AlbumSig : ADTSig :=
            : unit                             -> rep,
       Method "AddPhoto"
            : rep x (AlbumSchema#PHOTOS)       -> rep x bool,
-      Method "AddUser"
-           : rep x (AlbumSchema#USERS)        -> rep x bool,
-      Method "PhotosByLocation"
-           : rep x (NatRange * NatRange)      -> rep x list (AlbumSchema#PHOTOS),
+      Method "AddPerson"
+           : rep x (AlbumSchema#PEOPLE)       -> rep x bool,
+      Method "PhotosByAgeRange"
+           : rep x (nat * nat)                -> rep x list (AlbumSchema#PHOTOS),
       Method "PhotosByTags"
-           : rep x list string                -> rep x list (AlbumSchema#PHOTOS),
-      Method "PhotosByUploader"
-           : rep x string                     -> rep x list (AlbumSchema#PHOTOS)
+           : rep x list string                -> rep x list (AlbumSchema#PHOTOS)
     }.
 
 Definition AlbumSpec : ADT AlbumSig :=
@@ -60,26 +47,19 @@ Definition AlbumSpec : ADT AlbumSig :=
     update "AddPhoto" (photo : AlbumSchema#PHOTOS) : bool :=
       Insert photo into PHOTOS,
 
-    update "AddUser" (user : AlbumSchema#USERS) : bool :=
-      Insert user into USERS,
+    update "AddPerson" (person : AlbumSchema#PEOPLE) : bool :=
+      Insert person into PEOPLE,
 
-    query "PhotosByLocation" (ranges : NatRange * NatRange) : list (AlbumSchema#PHOTOS) :=
-      (* let (range_latitude, range_longitude) := ranges in *)
+    query "PhotosByAgeRange" (range : nat * nat) : list (AlbumSchema#PHOTOS) :=
       For (photo in PHOTOS)
-          Where (InRange photo!LATITUDE (fst ranges) /\
-                 InRange photo!LONGITUDE (snd ranges))
+          (person in PEOPLE)
+          Where (person!NAME = photo!NAME)
+          Where (InRange person!AGE range)
           Return photo,
           
     query "PhotosByTags" (search_tags : list string) : list (AlbumSchema#PHOTOS) :=
       For (photo in PHOTOS)
           Where (IncludedIn search_tags photo!TAGS)
-          Return photo,
-
-    query "PhotosByUploader" (uploader : string) : list (AlbumSchema#PHOTOS) :=
-      For (user in USERS)
-          (photo in PHOTOS)
-          Where (user!NAME = uploader)
-          Where (photo!USER_ID = user!USER_ID)
           Return photo
 }.
 
@@ -90,26 +70,22 @@ Proof.
 
   start honing QueryStructure.
 
-  make simple indexes using [[(RangeIndex, LATITUDE)]; [(EqualityIndex, NAME)]].
+  make simple indexes using [[(EqualityIndex, NAME); (InclusionIndex, TAGS)]; [(RangeIndex, AGE)]].
 
   hone constructor "Init".
   { initializer. }
 
-  hone method "PhotosByLocation".
-  { observer. }
-    
   hone method "PhotosByTags".
   { observer. }
 
-  hone method "PhotosByUploader".
+  hone method "PhotosByAgeRange".
   { observer. }
 
   hone method "AddPhoto".
   { insertion. }
 
-  hone method "AddUser".
+  hone method "AddPerson".
   { insertion. }
-
 
   FullySharpenQueryStructure AlbumSchema Index.
 
